add stronger wf condition to exp_rcd_cons

proof/uni_rcd/def_ott.v
@@ -52,12 +52,6 @@ Inductive dbind : Set :=
  | dbind_stvar_empty : dbind
  | dbind_typ (A:typ).
 
-Inductive abind : Set := 
- | abind_tvar_empty : abind
- | abind_stvar_empty : abind
- | abind_etvar_empty : abind
- | abind_var_typ (A:typ).
-
 Inductive work : Set := 
  | work_infer (e:exp) (cs:conts)
  | work_check (e:exp) (A:typ)
@@ -76,7 +70,18 @@ Inductive work : Set :=
  | work_applys (cs:conts) (A:typ)
  | work_applyd (cd:contd) (A:typ) (B:typ).
 
+Inductive abind : Set := 
+ | abind_tvar_empty : abind
+ | abind_stvar_empty : abind
+ | abind_etvar_empty : abind
+ | abind_var_typ (A:typ).
+
 Definition denv : Set := list (atom*dbind).
+
+Inductive dworklist : Set := 
+ | dworklist_empty : dworklist
+ | dworklist_cons_var (Ω:dworklist) (X:typvar) (db:dbind)
+ | dworklist_cons_work (Ω:dworklist) (w:work).
 
 Definition aenv : Set := list (atom*abind).
 
@@ -84,11 +89,6 @@ Inductive aworklist : Set :=
  | aworklist_empty : aworklist
  | aworklist_cons_var (Γ:aworklist) (X:typvar) (ab:abind)
  | aworklist_cons_work (Γ:aworklist) (w:work).
-
-Inductive dworklist : Set := 
- | dworklist_empty : dworklist
- | dworklist_cons_var (Ω:dworklist) (X:typvar) (db:dbind)
- | dworklist_cons_work (Ω:dworklist) (w:work).
 
 (* EXPERIMENTAL *)
 (** auxiliary functions on the new list types *)
@@ -319,21 +319,6 @@ Fixpoint close_typ_wrt_typ_rec (k:nat) (A_5:var) (A__6:typ) {struct A__6}: typ :
   | (typ_label l) => typ_label l
 end.
 
-Fixpoint close_exp_wrt_typ_rec (k:nat) (A_5:var) (e_5:exp) {struct e_5}: exp :=
-  match e_5 with
-  | exp_unit => exp_unit 
-  | (exp_var_b nat) => exp_var_b nat
-  | (exp_var_f x) => exp_var_f x
-  | (exp_abs e) => exp_abs (close_exp_wrt_typ_rec k A_5 e)
-  | (exp_app e1 e2) => exp_app (close_exp_wrt_typ_rec k A_5 e1) (close_exp_wrt_typ_rec k A_5 e2)
-  | (exp_tabs e) => exp_tabs (close_exp_wrt_typ_rec (S k) A_5 e)
-  | (exp_tapp e A) => exp_tapp (close_exp_wrt_typ_rec k A_5 e) (close_typ_wrt_typ_rec k A_5 A)
-  | (exp_anno e A) => exp_anno (close_exp_wrt_typ_rec k A_5 e) (close_typ_wrt_typ_rec k A_5 A)
-  | (exp_rcd_single l e) => exp_rcd_single l (close_exp_wrt_typ_rec k A_5 e)
-  | (exp_rcd_cons l e1 e2) => exp_rcd_cons l (close_exp_wrt_typ_rec k A_5 e1) (close_exp_wrt_typ_rec k A_5 e2)
-  | (exp_rcd_proj e l) => exp_rcd_proj (close_exp_wrt_typ_rec k A_5 e) l
-end.
-
 Fixpoint close_exp_wrt_exp_rec (k:nat) (e_5:var) (e__6:exp) {struct e__6}: exp :=
   match e__6 with
   | exp_unit => exp_unit 
@@ -352,23 +337,19 @@ Fixpoint close_exp_wrt_exp_rec (k:nat) (e_5:var) (e__6:exp) {struct e__6}: exp :
   | (exp_rcd_proj e l) => exp_rcd_proj (close_exp_wrt_exp_rec k e_5 e) l
 end.
 
-Fixpoint close_conts_wrt_typ_rec (k:nat) (A_5:var) (cs5:conts) {struct cs5}: conts :=
-  match cs5 with
-  | (conts_infabs cd) => conts_infabs (close_contd_wrt_typ_rec k A_5 cd)
-  | (conts_inftapp A cs) => conts_inftapp (close_typ_wrt_typ_rec k A_5 A) (close_conts_wrt_typ_rec k A_5 cs)
-  | (conts_inftappunion A1 A2 cs) => conts_inftappunion (close_typ_wrt_typ_rec k A_5 A1) (close_typ_wrt_typ_rec k A_5 A2) (close_conts_wrt_typ_rec k A_5 cs)
-  | (conts_unioninftapp A2 cs) => conts_unioninftapp (close_typ_wrt_typ_rec k A_5 A2) (close_conts_wrt_typ_rec k A_5 cs)
-  | (conts_infrcdsingle l cs) => conts_infrcdsingle l (close_conts_wrt_typ_rec k A_5 cs)
-  | (conts_infrcdconsintersection l e cs) => conts_infrcdconsintersection l (close_exp_wrt_typ_rec k A_5 e) (close_conts_wrt_typ_rec k A_5 cs)
-  | (conts_intersectioninfrcdcons A cs) => conts_intersectioninfrcdcons (close_typ_wrt_typ_rec k A_5 A) (close_conts_wrt_typ_rec k A_5 cs)
-  | (conts_sub A) => conts_sub (close_typ_wrt_typ_rec k A_5 A)
-end
-with close_contd_wrt_typ_rec (k:nat) (A5:var) (cd5:contd) {struct cd5}: contd :=
-  match cd5 with
-  | (contd_infabsunion A cd) => contd_infabsunion (close_typ_wrt_typ_rec k A5 A) (close_contd_wrt_typ_rec k A5 cd)
-  | (contd_infapp e cs) => contd_infapp (close_exp_wrt_typ_rec k A5 e) (close_conts_wrt_typ_rec k A5 cs)
-  | (contd_infproj A cs) => contd_infproj (close_typ_wrt_typ_rec k A5 A) (close_conts_wrt_typ_rec k A5 cs)
-  | (contd_unioninfabs A B cd) => contd_unioninfabs (close_typ_wrt_typ_rec k A5 A) (close_typ_wrt_typ_rec k A5 B) (close_contd_wrt_typ_rec k A5 cd)
+Fixpoint close_exp_wrt_typ_rec (k:nat) (A_5:var) (e_5:exp) {struct e_5}: exp :=
+  match e_5 with
+  | exp_unit => exp_unit 
+  | (exp_var_b nat) => exp_var_b nat
+  | (exp_var_f x) => exp_var_f x
+  | (exp_abs e) => exp_abs (close_exp_wrt_typ_rec k A_5 e)
+  | (exp_app e1 e2) => exp_app (close_exp_wrt_typ_rec k A_5 e1) (close_exp_wrt_typ_rec k A_5 e2)
+  | (exp_tabs e) => exp_tabs (close_exp_wrt_typ_rec (S k) A_5 e)
+  | (exp_tapp e A) => exp_tapp (close_exp_wrt_typ_rec k A_5 e) (close_typ_wrt_typ_rec k A_5 A)
+  | (exp_anno e A) => exp_anno (close_exp_wrt_typ_rec k A_5 e) (close_typ_wrt_typ_rec k A_5 A)
+  | (exp_rcd_single l e) => exp_rcd_single l (close_exp_wrt_typ_rec k A_5 e)
+  | (exp_rcd_cons l e1 e2) => exp_rcd_cons l (close_exp_wrt_typ_rec k A_5 e1) (close_exp_wrt_typ_rec k A_5 e2)
+  | (exp_rcd_proj e l) => exp_rcd_proj (close_exp_wrt_typ_rec k A_5 e) l
 end.
 
 Fixpoint close_contd_wrt_exp_rec (k:nat) (e5:var) (cd5:contd) {struct cd5}: contd :=
@@ -388,6 +369,52 @@ with close_conts_wrt_exp_rec (k:nat) (e5:var) (cs5:conts) {struct cs5}: conts :=
   | (conts_infrcdconsintersection l e cs) => conts_infrcdconsintersection l (close_exp_wrt_exp_rec k e5 e) (close_conts_wrt_exp_rec k e5 cs)
   | (conts_intersectioninfrcdcons A cs) => conts_intersectioninfrcdcons A (close_conts_wrt_exp_rec k e5 cs)
   | (conts_sub A) => conts_sub A
+end.
+
+Fixpoint close_contd_wrt_typ_rec (k:nat) (A5:var) (cd5:contd) {struct cd5}: contd :=
+  match cd5 with
+  | (contd_infabsunion A cd) => contd_infabsunion (close_typ_wrt_typ_rec k A5 A) (close_contd_wrt_typ_rec k A5 cd)
+  | (contd_infapp e cs) => contd_infapp (close_exp_wrt_typ_rec k A5 e) (close_conts_wrt_typ_rec k A5 cs)
+  | (contd_infproj A cs) => contd_infproj (close_typ_wrt_typ_rec k A5 A) (close_conts_wrt_typ_rec k A5 cs)
+  | (contd_unioninfabs A B cd) => contd_unioninfabs (close_typ_wrt_typ_rec k A5 A) (close_typ_wrt_typ_rec k A5 B) (close_contd_wrt_typ_rec k A5 cd)
+end
+with close_conts_wrt_typ_rec (k:nat) (A_5:var) (cs5:conts) {struct cs5}: conts :=
+  match cs5 with
+  | (conts_infabs cd) => conts_infabs (close_contd_wrt_typ_rec k A_5 cd)
+  | (conts_inftapp A cs) => conts_inftapp (close_typ_wrt_typ_rec k A_5 A) (close_conts_wrt_typ_rec k A_5 cs)
+  | (conts_inftappunion A1 A2 cs) => conts_inftappunion (close_typ_wrt_typ_rec k A_5 A1) (close_typ_wrt_typ_rec k A_5 A2) (close_conts_wrt_typ_rec k A_5 cs)
+  | (conts_unioninftapp A2 cs) => conts_unioninftapp (close_typ_wrt_typ_rec k A_5 A2) (close_conts_wrt_typ_rec k A_5 cs)
+  | (conts_infrcdsingle l cs) => conts_infrcdsingle l (close_conts_wrt_typ_rec k A_5 cs)
+  | (conts_infrcdconsintersection l e cs) => conts_infrcdconsintersection l (close_exp_wrt_typ_rec k A_5 e) (close_conts_wrt_typ_rec k A_5 cs)
+  | (conts_intersectioninfrcdcons A cs) => conts_intersectioninfrcdcons (close_typ_wrt_typ_rec k A_5 A) (close_conts_wrt_typ_rec k A_5 cs)
+  | (conts_sub A) => conts_sub (close_typ_wrt_typ_rec k A_5 A)
+end.
+
+Definition close_work_wrt_exp_rec (k:nat) (e5:var) (w5:work) : work :=
+  match w5 with
+  | (work_infer e cs) => work_infer (close_exp_wrt_exp_rec k e5 e) (close_conts_wrt_exp_rec k e5 cs)
+  | (work_check e A) => work_check (close_exp_wrt_exp_rec k e5 e) A
+  | (work_infabs A cd) => work_infabs A (close_contd_wrt_exp_rec k e5 cd)
+  | (work_infabsunion A1 B1 A2 cd) => work_infabsunion A1 B1 A2 (close_contd_wrt_exp_rec k e5 cd)
+  | (work_infapp A B e cs) => work_infapp A B (close_exp_wrt_exp_rec k e5 e) (close_conts_wrt_exp_rec k e5 cs)
+  | (work_infproj A B C cs) => work_infproj A B C (close_conts_wrt_exp_rec k e5 cs)
+  | (work_infrcdsingle l A cs) => work_infrcdsingle l A (close_conts_wrt_exp_rec k e5 cs)
+  | (work_infrcdconsintersection l A e cs) => work_infrcdconsintersection l A (close_exp_wrt_exp_rec k e5 e) (close_conts_wrt_exp_rec k e5 cs)
+  | (work_intersectioninfrcdcons A1 A2 cs) => work_intersectioninfrcdcons A1 A2 (close_conts_wrt_exp_rec k e5 cs)
+  | (work_inftapp A1 A2 cs) => work_inftapp A1 A2 (close_conts_wrt_exp_rec k e5 cs)
+  | (work_sub A1 A2) => work_sub A1 A2
+  | (work_inftappunion A1 A2 B cs) => work_inftappunion A1 A2 B (close_conts_wrt_exp_rec k e5 cs)
+  | (work_unioninftapp A1 A2 cs) => work_unioninftapp A1 A2 (close_conts_wrt_exp_rec k e5 cs)
+  | (work_unioninfabs A1 B1 A2 B2 cd) => work_unioninfabs A1 B1 A2 B2 (close_contd_wrt_exp_rec k e5 cd)
+  | (work_applys cs A) => work_applys (close_conts_wrt_exp_rec k e5 cs) A
+  | (work_applyd cd A B) => work_applyd (close_contd_wrt_exp_rec k e5 cd) A B
+end.
+
+Definition close_dbind_wrt_typ_rec (k:nat) (A5:var) (db5:dbind) : dbind :=
+  match db5 with
+  | dbind_tvar_empty => dbind_tvar_empty 
+  | dbind_stvar_empty => dbind_stvar_empty 
+  | (dbind_typ A) => dbind_typ (close_typ_wrt_typ_rec k A5 A)
 end.
 
 Definition close_work_wrt_typ_rec (k:nat) (A_5:var) (w5:work) : work :=
@@ -418,52 +445,11 @@ Definition close_abind_wrt_typ_rec (k:nat) (A5:var) (ab5:abind) : abind :=
   | (abind_var_typ A) => abind_var_typ (close_typ_wrt_typ_rec k A5 A)
 end.
 
-Definition close_work_wrt_exp_rec (k:nat) (e5:var) (w5:work) : work :=
-  match w5 with
-  | (work_infer e cs) => work_infer (close_exp_wrt_exp_rec k e5 e) (close_conts_wrt_exp_rec k e5 cs)
-  | (work_check e A) => work_check (close_exp_wrt_exp_rec k e5 e) A
-  | (work_infabs A cd) => work_infabs A (close_contd_wrt_exp_rec k e5 cd)
-  | (work_infabsunion A1 B1 A2 cd) => work_infabsunion A1 B1 A2 (close_contd_wrt_exp_rec k e5 cd)
-  | (work_infapp A B e cs) => work_infapp A B (close_exp_wrt_exp_rec k e5 e) (close_conts_wrt_exp_rec k e5 cs)
-  | (work_infproj A B C cs) => work_infproj A B C (close_conts_wrt_exp_rec k e5 cs)
-  | (work_infrcdsingle l A cs) => work_infrcdsingle l A (close_conts_wrt_exp_rec k e5 cs)
-  | (work_infrcdconsintersection l A e cs) => work_infrcdconsintersection l A (close_exp_wrt_exp_rec k e5 e) (close_conts_wrt_exp_rec k e5 cs)
-  | (work_intersectioninfrcdcons A1 A2 cs) => work_intersectioninfrcdcons A1 A2 (close_conts_wrt_exp_rec k e5 cs)
-  | (work_inftapp A1 A2 cs) => work_inftapp A1 A2 (close_conts_wrt_exp_rec k e5 cs)
-  | (work_sub A1 A2) => work_sub A1 A2
-  | (work_inftappunion A1 A2 B cs) => work_inftappunion A1 A2 B (close_conts_wrt_exp_rec k e5 cs)
-  | (work_unioninftapp A1 A2 cs) => work_unioninftapp A1 A2 (close_conts_wrt_exp_rec k e5 cs)
-  | (work_unioninfabs A1 B1 A2 B2 cd) => work_unioninfabs A1 B1 A2 B2 (close_contd_wrt_exp_rec k e5 cd)
-  | (work_applys cs A) => work_applys (close_conts_wrt_exp_rec k e5 cs) A
-  | (work_applyd cd A B) => work_applyd (close_contd_wrt_exp_rec k e5 cd) A B
-end.
-
-Definition close_dbind_wrt_typ_rec (k:nat) (A5:var) (db5:dbind) : dbind :=
-  match db5 with
-  | dbind_tvar_empty => dbind_tvar_empty 
-  | dbind_stvar_empty => dbind_stvar_empty 
-  | (dbind_typ A) => dbind_typ (close_typ_wrt_typ_rec k A5 A)
-end.
-
-Fixpoint close_aworklist_wrt_typ_rec (k:nat) (A5:var) (Γ_5:aworklist) {struct Γ_5}: aworklist :=
-  match Γ_5 with
-  | aworklist_empty => aworklist_empty 
-  | (aworklist_cons_var Γ X ab) => aworklist_cons_var (close_aworklist_wrt_typ_rec k A5 Γ) X (close_abind_wrt_typ_rec k A5 ab)
-  | (aworklist_cons_work Γ w) => aworklist_cons_work (close_aworklist_wrt_typ_rec k A5 Γ) (close_work_wrt_typ_rec k A5 w)
-end.
-
 Fixpoint close_aworklist_wrt_exp_rec (k:nat) (e5:var) (Γ_5:aworklist) {struct Γ_5}: aworklist :=
   match Γ_5 with
   | aworklist_empty => aworklist_empty 
   | (aworklist_cons_var Γ X ab) => aworklist_cons_var (close_aworklist_wrt_exp_rec k e5 Γ) X ab
   | (aworklist_cons_work Γ w) => aworklist_cons_work (close_aworklist_wrt_exp_rec k e5 Γ) (close_work_wrt_exp_rec k e5 w)
-end.
-
-Fixpoint close_dworklist_wrt_exp_rec (k:nat) (e5:var) (Ω5:dworklist) {struct Ω5}: dworklist :=
-  match Ω5 with
-  | dworklist_empty => dworklist_empty 
-  | (dworklist_cons_var Ω X db) => dworklist_cons_var (close_dworklist_wrt_exp_rec k e5 Ω) X db
-  | (dworklist_cons_work Ω w) => dworklist_cons_work (close_dworklist_wrt_exp_rec k e5 Ω) (close_work_wrt_exp_rec k e5 w)
 end.
 
 Fixpoint close_dworklist_wrt_typ_rec (k:nat) (A5:var) (Ω5:dworklist) {struct Ω5}: dworklist :=
@@ -473,35 +459,49 @@ Fixpoint close_dworklist_wrt_typ_rec (k:nat) (A5:var) (Ω5:dworklist) {struct Ω
   | (dworklist_cons_work Ω w) => dworklist_cons_work (close_dworklist_wrt_typ_rec k A5 Ω) (close_work_wrt_typ_rec k A5 w)
 end.
 
-Definition close_aworklist_wrt_typ Γ_5 A5 := close_aworklist_wrt_typ_rec 0 Γ_5 A5.
+Fixpoint close_dworklist_wrt_exp_rec (k:nat) (e5:var) (Ω5:dworklist) {struct Ω5}: dworklist :=
+  match Ω5 with
+  | dworklist_empty => dworklist_empty 
+  | (dworklist_cons_var Ω X db) => dworklist_cons_var (close_dworklist_wrt_exp_rec k e5 Ω) X db
+  | (dworklist_cons_work Ω w) => dworklist_cons_work (close_dworklist_wrt_exp_rec k e5 Ω) (close_work_wrt_exp_rec k e5 w)
+end.
 
-Definition close_contd_wrt_typ cd5 A5 := close_contd_wrt_typ_rec 0 cd5 A5.
-
-Definition close_work_wrt_typ w5 A_5 := close_work_wrt_typ_rec 0 w5 A_5.
-
-Definition close_aworklist_wrt_exp Γ_5 e5 := close_aworklist_wrt_exp_rec 0 Γ_5 e5.
-
-Definition close_abind_wrt_typ ab5 A5 := close_abind_wrt_typ_rec 0 ab5 A5.
-
-Definition close_conts_wrt_exp cs5 e5 := close_conts_wrt_exp_rec 0 cs5 e5.
-
-Definition close_dworklist_wrt_exp Ω5 e5 := close_dworklist_wrt_exp_rec 0 Ω5 e5.
+Fixpoint close_aworklist_wrt_typ_rec (k:nat) (A5:var) (Γ_5:aworklist) {struct Γ_5}: aworklist :=
+  match Γ_5 with
+  | aworklist_empty => aworklist_empty 
+  | (aworklist_cons_var Γ X ab) => aworklist_cons_var (close_aworklist_wrt_typ_rec k A5 Γ) X (close_abind_wrt_typ_rec k A5 ab)
+  | (aworklist_cons_work Γ w) => aworklist_cons_work (close_aworklist_wrt_typ_rec k A5 Γ) (close_work_wrt_typ_rec k A5 w)
+end.
 
 Definition close_dbind_wrt_typ db5 A5 := close_dbind_wrt_typ_rec 0 db5 A5.
 
-Definition close_exp_wrt_typ e_5 A_5 := close_exp_wrt_typ_rec 0 e_5 A_5.
+Definition close_exp_wrt_exp e__6 e_5 := close_exp_wrt_exp_rec 0 e__6 e_5.
+
+Definition close_aworklist_wrt_exp Γ_5 e5 := close_aworklist_wrt_exp_rec 0 Γ_5 e5.
+
+Definition close_work_wrt_typ w5 A_5 := close_work_wrt_typ_rec 0 w5 A_5.
+
+Definition close_work_wrt_exp w5 e5 := close_work_wrt_exp_rec 0 w5 e5.
+
+Definition close_conts_wrt_exp cs5 e5 := close_conts_wrt_exp_rec 0 cs5 e5.
+
+Definition close_abind_wrt_typ ab5 A5 := close_abind_wrt_typ_rec 0 ab5 A5.
 
 Definition close_conts_wrt_typ cs5 A_5 := close_conts_wrt_typ_rec 0 cs5 A_5.
+
+Definition close_dworklist_wrt_typ Ω5 A5 := close_dworklist_wrt_typ_rec 0 Ω5 A5.
+
+Definition close_exp_wrt_typ e_5 A_5 := close_exp_wrt_typ_rec 0 e_5 A_5.
+
+Definition close_dworklist_wrt_exp Ω5 e5 := close_dworklist_wrt_exp_rec 0 Ω5 e5.
 
 Definition close_typ_wrt_typ A__6 A_5 := close_typ_wrt_typ_rec 0 A__6 A_5.
 
 Definition close_contd_wrt_exp cd5 e5 := close_contd_wrt_exp_rec 0 cd5 e5.
 
-Definition close_work_wrt_exp w5 e5 := close_work_wrt_exp_rec 0 w5 e5.
+Definition close_contd_wrt_typ cd5 A5 := close_contd_wrt_typ_rec 0 cd5 A5.
 
-Definition close_dworklist_wrt_typ Ω5 A5 := close_dworklist_wrt_typ_rec 0 Ω5 A5.
-
-Definition close_exp_wrt_exp e__6 e_5 := close_exp_wrt_exp_rec 0 e__6 e_5.
+Definition close_aworklist_wrt_typ Γ_5 A5 := close_aworklist_wrt_typ_rec 0 Γ_5 A5.
 
 (** terms are locally-closed pre-terms *)
 (** definitions *)
@@ -630,18 +630,6 @@ Inductive lc_dbind : dbind -> Prop :=    (* defn lc_dbind *)
      (lc_typ A) ->
      (lc_dbind (dbind_typ A)).
 
-(* defns LC_abind *)
-Inductive lc_abind : abind -> Prop :=    (* defn lc_abind *)
- | lc_abind_tvar_empty : 
-     (lc_abind abind_tvar_empty)
- | lc_abind_stvar_empty : 
-     (lc_abind abind_stvar_empty)
- | lc_abind_etvar_empty : 
-     (lc_abind abind_etvar_empty)
- | lc_abind_var_typ : forall (A:typ),
-     (lc_typ A) ->
-     (lc_abind (abind_var_typ A)).
-
 (* defns LC_work *)
 Inductive lc_work : work -> Prop :=    (* defn lc_work *)
  | lc_work_infer : forall (e:exp) (cs:conts),
@@ -725,18 +713,17 @@ Inductive lc_work : work -> Prop :=    (* defn lc_work *)
      (lc_typ B) ->
      (lc_work (work_applyd cd A B)).
 
-(* defns LC_aworklist *)
-Inductive lc_aworklist : aworklist -> Prop :=    (* defn lc_aworklist *)
- | lc_aworklist_empty : 
-     (lc_aworklist aworklist_empty)
- | lc_aworklist_cons_var : forall (Γ:aworklist) (X:typvar) (ab:abind),
-     (lc_aworklist Γ) ->
-     (lc_abind ab) ->
-     (lc_aworklist (aworklist_cons_var Γ X ab))
- | lc_aworklist_cons_work : forall (Γ:aworklist) (w:work),
-     (lc_aworklist Γ) ->
-     (lc_work w) ->
-     (lc_aworklist (aworklist_cons_work Γ w)).
+(* defns LC_abind *)
+Inductive lc_abind : abind -> Prop :=    (* defn lc_abind *)
+ | lc_abind_tvar_empty : 
+     (lc_abind abind_tvar_empty)
+ | lc_abind_stvar_empty : 
+     (lc_abind abind_stvar_empty)
+ | lc_abind_etvar_empty : 
+     (lc_abind abind_etvar_empty)
+ | lc_abind_var_typ : forall (A:typ),
+     (lc_typ A) ->
+     (lc_abind (abind_var_typ A)).
 
 (* defns LC_dworklist *)
 Inductive lc_dworklist : dworklist -> Prop :=    (* defn lc_dworklist *)
@@ -750,6 +737,19 @@ Inductive lc_dworklist : dworklist -> Prop :=    (* defn lc_dworklist *)
      (lc_dworklist Ω) ->
      (lc_work w) ->
      (lc_dworklist (dworklist_cons_work Ω w)).
+
+(* defns LC_aworklist *)
+Inductive lc_aworklist : aworklist -> Prop :=    (* defn lc_aworklist *)
+ | lc_aworklist_empty : 
+     (lc_aworklist aworklist_empty)
+ | lc_aworklist_cons_var : forall (Γ:aworklist) (X:typvar) (ab:abind),
+     (lc_aworklist Γ) ->
+     (lc_abind ab) ->
+     (lc_aworklist (aworklist_cons_var Γ X ab))
+ | lc_aworklist_cons_work : forall (Γ:aworklist) (w:work),
+     (lc_aworklist Γ) ->
+     (lc_work w) ->
+     (lc_aworklist (aworklist_cons_work Γ w)).
 (** free variables *)
 Fixpoint ftvar_in_typ (A_5:typ) : vars :=
   match A_5 with
@@ -999,13 +999,6 @@ with subst_exp_in_conts (e5:exp) (x5:expvar) (cs5:conts) {struct cs5} : conts :=
   | (conts_sub A) => conts_sub A
 end.
 
-Definition subst_typ_in_dbind (A5:typ) (X5:typvar) (db5:dbind) : dbind :=
-  match db5 with
-  | dbind_tvar_empty => dbind_tvar_empty 
-  | dbind_stvar_empty => dbind_stvar_empty 
-  | (dbind_typ A) => dbind_typ (subst_typ_in_typ A5 X5 A)
-end.
-
 Definition subst_typ_in_work (A_5:typ) (X5:typvar) (w5:work) : work :=
   match w5 with
   | (work_infer e cs) => work_infer (subst_typ_in_exp A_5 X5 e) (subst_typ_in_conts A_5 X5 cs)
@@ -1024,6 +1017,21 @@ Definition subst_typ_in_work (A_5:typ) (X5:typvar) (w5:work) : work :=
   | (work_unioninfabs A1 B1 A2 B2 cd) => work_unioninfabs (subst_typ_in_typ A_5 X5 A1) (subst_typ_in_typ A_5 X5 B1) (subst_typ_in_typ A_5 X5 A2) (subst_typ_in_typ A_5 X5 B2) (subst_typ_in_contd A_5 X5 cd)
   | (work_applys cs A) => work_applys (subst_typ_in_conts A_5 X5 cs) (subst_typ_in_typ A_5 X5 A)
   | (work_applyd cd A B) => work_applyd (subst_typ_in_contd A_5 X5 cd) (subst_typ_in_typ A_5 X5 A) (subst_typ_in_typ A_5 X5 B)
+end.
+
+Definition subst_typ_in_abind (A5:typ) (X5:typvar) (ab5:abind) : abind :=
+  match ab5 with
+  | abind_tvar_empty => abind_tvar_empty 
+  | abind_stvar_empty => abind_stvar_empty 
+  | abind_etvar_empty => abind_etvar_empty 
+  | (abind_var_typ A) => abind_var_typ (subst_typ_in_typ A5 X5 A)
+end.
+
+Definition subst_typ_in_dbind (A5:typ) (X5:typvar) (db5:dbind) : dbind :=
+  match db5 with
+  | dbind_tvar_empty => dbind_tvar_empty 
+  | dbind_stvar_empty => dbind_stvar_empty 
+  | (dbind_typ A) => dbind_typ (subst_typ_in_typ A5 X5 A)
 end.
 
 Definition subst_exp_in_work (e5:exp) (x5:expvar) (w5:work) : work :=
@@ -1046,12 +1054,11 @@ Definition subst_exp_in_work (e5:exp) (x5:expvar) (w5:work) : work :=
   | (work_applyd cd A B) => work_applyd (subst_exp_in_contd e5 x5 cd) A B
 end.
 
-Definition subst_typ_in_abind (A5:typ) (X5:typvar) (ab5:abind) : abind :=
-  match ab5 with
-  | abind_tvar_empty => abind_tvar_empty 
-  | abind_stvar_empty => abind_stvar_empty 
-  | abind_etvar_empty => abind_etvar_empty 
-  | (abind_var_typ A) => abind_var_typ (subst_typ_in_typ A5 X5 A)
+Fixpoint subst_typ_in_aworklist (A5:typ) (X5:typvar) (Γ_5:aworklist) {struct Γ_5} : aworklist :=
+  match Γ_5 with
+  | aworklist_empty => aworklist_empty 
+  | (aworklist_cons_var Γ X ab) => aworklist_cons_var (subst_typ_in_aworklist A5 X5 Γ) X (subst_typ_in_abind A5 X5 ab)
+  | (aworklist_cons_work Γ w) => aworklist_cons_work (subst_typ_in_aworklist A5 X5 Γ) (subst_typ_in_work A5 X5 w)
 end.
 
 Fixpoint subst_typ_in_dworklist (A5:typ) (X5:typvar) (Ω5:dworklist) {struct Ω5} : dworklist :=
@@ -1066,13 +1073,6 @@ Fixpoint subst_exp_in_dworklist (e5:exp) (x5:expvar) (Ω5:dworklist) {struct Ω5
   | dworklist_empty => dworklist_empty 
   | (dworklist_cons_var Ω X db) => dworklist_cons_var (subst_exp_in_dworklist e5 x5 Ω) X db
   | (dworklist_cons_work Ω w) => dworklist_cons_work (subst_exp_in_dworklist e5 x5 Ω) (subst_exp_in_work e5 x5 w)
-end.
-
-Fixpoint subst_typ_in_aworklist (A5:typ) (X5:typvar) (Γ_5:aworklist) {struct Γ_5} : aworklist :=
-  match Γ_5 with
-  | aworklist_empty => aworklist_empty 
-  | (aworklist_cons_var Γ X ab) => aworklist_cons_var (subst_typ_in_aworklist A5 X5 Γ) X (subst_typ_in_abind A5 X5 ab)
-  | (aworklist_cons_work Γ w) => aworklist_cons_work (subst_typ_in_aworklist A5 X5 Γ) (subst_typ_in_work A5 X5 w)
 end.
 
 Fixpoint subst_exp_in_aworklist (e5:exp) (x5:expvar) (Γ_5:aworklist) {struct Γ_5} : aworklist :=
@@ -1102,6 +1102,16 @@ Fixpoint awl_to_aenv (Γ : aworklist) : aenv :=
 
 
 (** definitions *)
+
+(* defns J_is_exp_rcd *)
+Inductive is_exp_rcd : exp -> Prop :=    (* defn is_exp_rcd *)
+ | is_exp_rcd__single_ : forall (l:label) (e1:exp),
+     lc_exp e1 ->
+     is_exp_rcd (exp_rcd_single l e1)
+ | is_exp_rcd__cons : forall (l:label) (e1 e2:exp),
+     lc_exp e1 ->
+     is_exp_rcd e2 ->
+     is_exp_rcd (exp_rcd_cons l e1 e2).
 
 (* defns J_strong_in *)
 Inductive s_in : typvar -> typ -> Prop :=    (* defn s_in *)
@@ -1243,6 +1253,7 @@ Inductive d_wf_exp : denv -> exp -> Prop :=    (* defn d_wf_exp *)
  | d_wf_exp__rcd_cons : forall (Ψ:denv) (l:label) (e1 e2:exp),
      d_wf_exp Ψ e1 ->
      d_wf_exp Ψ e2 ->
+     is_exp_rcd e2 ->
      d_wf_exp Ψ (exp_rcd_cons l e1 e2)
  | d_wf_exp__rcd_projs : forall (Ψ:denv) (e:exp) (l:label),
      d_wf_exp Ψ e ->
@@ -1565,6 +1576,7 @@ Inductive a_wf_exp : aenv -> exp -> Prop :=    (* defn a_wf_exp *)
  | a_wf_exp__rcd_cons : forall (Σ:aenv) (l:label) (e1 e2:exp),
      a_wf_exp Σ e1 ->
      a_wf_exp Σ e2 ->
+     is_exp_rcd e2 ->
      a_wf_exp Σ (exp_rcd_cons l e1 e2)
  | a_wf_exp__rcd_projs : forall (Σ:aenv) (e:exp) (l:label),
      a_wf_exp Σ e ->
@@ -1790,6 +1802,6 @@ Inductive a_wf_env : aenv -> Prop :=    (* defn a_wf_env *)
 
 
 (** infrastructure *)
-#[export] Hint Constructors s_in neq_abs d_wneq_all d_wf_typ d_wf_exp d_wf_tenv d_wf_env d_mono_typ d_wf_conts d_wf_contd d_wf_work d_wf_twl d_wf_wl a_wneq_all a_wf_typ a_mono_typ a_wf_exp a_wf_conts a_wf_contd a_wf_work a_wf_wwl a_wf_twl a_wf_wl a_wf_env lc_typ lc_exp lc_contd lc_conts lc_dbind lc_abind lc_work lc_aworklist lc_dworklist : core.
+#[export] Hint Constructors is_exp_rcd s_in neq_abs d_wneq_all d_wf_typ d_wf_exp d_wf_tenv d_wf_env d_mono_typ d_wf_conts d_wf_contd d_wf_work d_wf_twl d_wf_wl a_wneq_all a_wf_typ a_mono_typ a_wf_exp a_wf_conts a_wf_contd a_wf_work a_wf_wwl a_wf_twl a_wf_wl a_wf_env lc_typ lc_exp lc_contd lc_conts lc_dbind lc_work lc_abind lc_dworklist lc_aworklist : core.
 
 
